Modify specification style for Weierstrass curve point operations
The previous specifications proved that, assuming none of the usual
degenerate cases, the results correspond to "canonical" Jacobian
operations, with specific encoding of the point at infinity as
(1,1,0). However, this canonical form seems to have little or no
implementation value and any interesting conclusions are excluded by
the exceptions in the precondition.

The new specifications are stated in terms of the mapping back to
affine form, for which any triple of the form (x,y,0) is treated as
the point at infinity. This already removes all special cases from
doubling and removes one of the four special cases from addition,
namely x + -x' = 0 where x' and x are projectively equivalent. The
new specifications are also perhaps a bit more compact and easily
understood.

arm/proofs/p256_montjmixadd.ml
@@ -1386,52 +1386,6 @@ let P256_MONTJMIXADD_EXEC = ARM_MK_EXEC_RULE p256_montjmixadd_mc;;
 (* Common supporting definitions and lemmas for component proofs.            *)
 (* ------------------------------------------------------------------------- *)
 
-let p_256 = new_definition `p_256 = 115792089210356248762697446949407573530086143415290314195533631308867097853951`;;
-
-let nistp256 = define
- `nistp256 =
-    (integer_mod_ring p_256,
-     ring_neg (integer_mod_ring p_256) (&3),
-     &b_256:int)`;;
-
-let nistp256_encode = new_definition
-  `nistp256_encode = montgomery_encode(256,p_256)`;;
-
-let nintlemma = prove
- (`&(num_of_int(x rem &p_256)) = x rem &p_256`,
-  MATCH_MP_TAC INT_OF_NUM_OF_INT THEN MATCH_MP_TAC INT_REM_POS THEN
-  REWRITE_TAC[INT_OF_NUM_EQ; p_256] THEN CONV_TAC NUM_REDUCE_CONV);;
-
-let unilemma0 = prove
- (`x = a MOD p_256 ==> x < p_256 /\ &x = &a rem &p_256`,
-  REWRITE_TAC[INT_OF_NUM_REM; p_256] THEN ARITH_TAC);;
-
-let unilemma1 = prove
- (`&x = a rem &p_256 ==> x < p_256 /\ &x = a rem &p_256`,
-  SIMP_TAC[GSYM INT_OF_NUM_LT; INT_LT_REM_EQ; p_256] THEN INT_ARITH_TAC);;
-
-let unilemma2 = prove
- (`X = num_of_int(x rem &p_256) ==> X < p_256 /\ &X = x rem &p_256`,
-  DISCH_THEN SUBST1_TAC THEN
-  REWRITE_TAC[GSYM INT_OF_NUM_LT; nintlemma; INT_LT_REM_EQ] THEN
-  REWRITE_TAC[INT_OF_NUM_LT; p_256] THEN CONV_TAC NUM_REDUCE_CONV);;
-
-let lemont = prove
- (`(&i * x * y) rem &p_256 = (&i * x rem &p_256 * y rem &p_256) rem &p_256`,
-  CONV_TAC INT_REM_DOWN_CONV THEN REWRITE_TAC[]);;
-
-let pumont = prove
- (`(&(inverse_mod p_256 (2 EXP 256)) *
-    (&2 pow 256 * x) rem &p_256 * (&2 pow 256 * y) rem &p_256) rem &p_256 =
-   (&2 pow 256 * x * y) rem &p_256`,
-  CONV_TAC INT_REM_DOWN_CONV THEN REWRITE_TAC[INT_REM_EQ] THEN
-  MATCH_MP_TAC(INTEGER_RULE
-   `(i * t:int == &1) (mod p)
-    ==> (i * (t * x) * (t * y) == t * x * y) (mod p)`) THEN
-  REWRITE_TAC[GSYM num_congruent; INT_OF_NUM_CLAUSES] THEN
-  REWRITE_TAC[INVERSE_MOD_LMUL_EQ; COPRIME_REXP; COPRIME_2; p_256] THEN
-  CONV_TAC NUM_REDUCE_CONV);;
-
 let lvs =
  ["x_1",[`X16`;`0`];
   "y_1",[`X16`;`32`];
@@ -1877,6 +1831,119 @@ let LOCAL_AMONTSQR_P256_TAC =
 (* Overall point operation proof.                                            *)
 (* ------------------------------------------------------------------------- *)
 
+let unilemma0 = prove
+ (`x = a MOD p_256 ==> x < p_256 /\ &x = &a rem &p_256`,
+  REWRITE_TAC[INT_OF_NUM_REM; p_256] THEN ARITH_TAC);;
+
+let unilemma1 = prove
+ (`&x = a rem &p_256 ==> x < p_256 /\ &x = a rem &p_256`,
+  SIMP_TAC[GSYM INT_OF_NUM_LT; INT_LT_REM_EQ; p_256] THEN INT_ARITH_TAC);;
+
+let lemont = prove
+ (`(&i * x * y) rem &p_256 = (&i * x rem &p_256 * y rem &p_256) rem &p_256`,
+  CONV_TAC INT_REM_DOWN_CONV THEN REWRITE_TAC[]);;
+
+let demont = prove
+ (`(&(NUMERAL n) * &x) rem &p_256 = (&(NUMERAL n) * &x rem &p_256) rem &p_256`,
+  CONV_TAC INT_REM_DOWN_CONV THEN REWRITE_TAC[]);;
+
+let pumont = prove
+ (`(&(inverse_mod p_256 (2 EXP 256)) *
+    (&2 pow 256 * x) rem &p_256 * (&2 pow 256 * y) rem &p_256) rem &p_256 =
+   (&2 pow 256 * x * y) rem &p_256`,
+  CONV_TAC INT_REM_DOWN_CONV THEN REWRITE_TAC[INT_REM_EQ] THEN
+  MATCH_MP_TAC(INTEGER_RULE
+   `(i * t:int == &1) (mod p)
+    ==> (i * (t * x) * (t * y) == t * x * y) (mod p)`) THEN
+  REWRITE_TAC[GSYM num_congruent; INT_OF_NUM_CLAUSES] THEN
+  REWRITE_TAC[INVERSE_MOD_LMUL_EQ; COPRIME_REXP; COPRIME_2; p_256] THEN
+  CONV_TAC NUM_REDUCE_CONV);;
+
+let dismont = prove
+ (`((&2 pow 256 * x) rem &p_256 + (&2 pow 256 * y) rem &p_256) rem &p_256 =
+   (&2 pow 256 * (x + y)) rem &p_256 /\
+   ((&2 pow 256 * x) rem &p_256 - (&2 pow 256 * y) rem &p_256) rem &p_256 =
+   (&2 pow 256 * (x - y)) rem &p_256 /\
+   (&(NUMERAL n) * (&2 pow 256 * x) rem &p_256) rem &p_256 =
+   (&2 pow 256 * (&(NUMERAL n) * x)) rem &p_256`,
+  REPEAT CONJ_TAC THEN CONV_TAC INT_REM_DOWN_CONV THEN
+  AP_THM_TAC THEN AP_TERM_TAC THEN INT_ARITH_TAC);;
+
+let unmont = prove
+ (`(&(inverse_mod p_256 (2 EXP 256)) * (&2 pow 256 * x) rem &p_256) rem &p_256 =
+   x rem &p_256`,
+  CONV_TAC INT_REM_DOWN_CONV THEN REWRITE_TAC[INT_REM_EQ] THEN
+  MATCH_MP_TAC(INTEGER_RULE
+   `(i * e:int == &1) (mod p) ==> (i * e * x == x) (mod p)`) THEN
+  REWRITE_TAC[INT_OF_NUM_CLAUSES; GSYM num_congruent; INVERSE_MOD_LMUL_EQ] THEN
+  REWRITE_TAC[COPRIME_REXP; COPRIME_2; p_256] THEN CONV_TAC NUM_REDUCE_CONV);;
+
+let unreplemma = prove
+ (`!x. x < p_256
+         ==> x =
+             (2 EXP 256 * (inverse_mod p_256 (2 EXP 256) * x) MOD p_256) MOD
+             p_256`,
+  REPEAT STRIP_TAC THEN CONV_TAC SYM_CONV THEN
+  ASM_REWRITE_TAC[MOD_UNIQUE] THEN
+  REWRITE_TAC[CONG] THEN CONV_TAC MOD_DOWN_CONV THEN
+  REWRITE_TAC[GSYM CONG] THEN MATCH_MP_TAC(NUMBER_RULE
+   `(i * e == 1) (mod p) ==> (i * e * x == x) (mod p)`) THEN
+  REWRITE_TAC[INVERSE_MOD_RMUL_EQ] THEN
+  REWRITE_TAC[COPRIME_REXP; COPRIME_2; p_256] THEN CONV_TAC NUM_REDUCE_CONV);;
+
+let weierstrass_of_affine_p256 = prove
+ (`weierstrass_of_jacobian (integer_mod_ring p_256)
+                           (x rem &p_256,y rem &p_256,&1 rem &p_256) =
+   SOME(x rem &p_256,y rem &p_256)`,
+  MP_TAC(ISPEC `integer_mod_ring p_256` RING_INV_1) THEN
+  REWRITE_TAC[weierstrass_of_jacobian; ring_div; INTEGER_MOD_RING_CLAUSES] THEN
+  REWRITE_TAC[p_256] THEN CONV_TAC INT_REDUCE_CONV THEN
+  SIMP_TAC[GSYM p_256; option_INJ; PAIR_EQ; INT_MUL_RID; INT_REM_REM]);;
+
+let weierstrass_of_jacobian_p256_add = prove
+ (`!P1 P2 x1 y1 z1 x2 y2 z2 x3 y3 z3.
+        ~(weierstrass_of_jacobian (integer_mod_ring p_256)
+           (x1 rem &p_256,y1 rem &p_256,z1 rem &p_256) =
+          weierstrass_of_jacobian (integer_mod_ring p_256)
+           (x2 rem &p_256,y2 rem &p_256,z2 rem &p_256)) /\
+        jacobian_add_unexceptional nistp256
+         (x1 rem &p_256,y1 rem &p_256,z1 rem &p_256)
+         (x2 rem &p_256,y2 rem &p_256,z2 rem &p_256) =
+        (x3 rem &p_256,y3 rem &p_256,z3 rem &p_256)
+        ==> weierstrass_of_jacobian (integer_mod_ring p_256)
+                (x1 rem &p_256,y1 rem &p_256,z1 rem &p_256) = P1 /\
+            weierstrass_of_jacobian (integer_mod_ring p_256)
+                (x2 rem &p_256,y2 rem &p_256,z2 rem &p_256) = P2
+            ==> weierstrass_of_jacobian (integer_mod_ring p_256)
+                  (x3 rem &p_256,y3 rem &p_256,z3 rem &p_256) =
+                group_mul p256_group P1 P2`,
+  REPEAT GEN_TAC THEN
+  DISCH_THEN(CONJUNCTS_THEN2 ASSUME_TAC (SUBST1_TAC o SYM)) THEN
+  DISCH_THEN(CONJUNCTS_THEN(SUBST1_TAC o SYM)) THEN
+  REWRITE_TAC[nistp256; P256_GROUP] THEN
+  MATCH_MP_TAC WEIERSTRASS_OF_JACOBIAN_ADD_UNEXCEPTIONAL THEN
+  REWRITE_TAC[CONJ_ASSOC] THEN CONJ_TAC THENL
+   [ALL_TAC;
+    W(MP_TAC o PART_MATCH (rand o rand) WEIERSTRASS_OF_JACOBIAN_EQ o
+      rand o snd) THEN
+    ASM_REWRITE_TAC[] THEN DISCH_THEN MATCH_MP_TAC] THEN
+  ASM_REWRITE_TAC[FIELD_INTEGER_MOD_RING; PRIME_P256] THEN
+  ASM_REWRITE_TAC[jacobian_point; INTEGER_MOD_RING_CHAR;
+                  INTEGER_MOD_RING_CLAUSES; IN_INTEGER_MOD_RING_CARRIER] THEN
+  REWRITE_TAC[INT_REM_POS_EQ; INT_LT_REM_EQ; GSYM INT_OF_NUM_CLAUSES] THEN
+  REWRITE_TAC[p_256; b_256] THEN CONV_TAC INT_REDUCE_CONV);;
+
+let represents_p256 = new_definition
+ `represents_p256 P (x,y,z) <=>
+        x < p_256 /\ y < p_256 /\ z < p_256 /\
+        weierstrass_of_jacobian (integer_mod_ring p_256)
+         (tripled (montgomery_decode (256,p_256)) (x,y,z)) = P`;;
+
+let represents2_p256 = new_definition
+ `represents2_p256 P (x,y) <=>
+        x < p_256 /\ y < p_256 /\
+        SOME(paired (montgomery_decode (256,p_256)) (x,y)) = P`;;
+
 let P256_MONTJMIXADD_CORRECT = time prove
  (`!p3 p1 t1 p2 t2 pc stackpointer.
         aligned 16 stackpointer /\
@@ -1892,18 +1959,11 @@ let P256_MONTJMIXADD_CORRECT = time prove
                   bignum_triple_from_memory (p1,4) s = t1 /\
                   bignum_pair_from_memory (p2,4) s = t2)
              (\s. read PC s = word (pc + 0x1528) /\
-                  (!x1 y1 z1 x2 y2 z2.
-                        ~(z1 = &0) /\ z2 = &1 /\
-                        ~(jacobian_eq (integer_mod_ring p_256)
-                                      (x1,y1,z1) (x2,y2,z2)) /\
-                        ~(jacobian_eq (integer_mod_ring p_256)
-                                      (jacobian_neg nistp256 (x1,y1,z1))
-                                      (x2,y2,z2)) /\
-                        t1 = tripled nistp256_encode (x1,y1,z1) /\
-                        t2 = paired nistp256_encode (x2,y2)
-                        ==> bignum_triple_from_memory(p3,4) s =
-                            tripled nistp256_encode
-                             (jacobian_add nistp256 (x1,y1,z1) (x2,y2,z2))))
+                  !P1 P2. represents_p256 P1 t1 /\
+                          represents2_p256 P2 t2 /\
+                          ~(P1 = NONE) /\ ~(P1 = P2)
+                          ==> represents_p256 (group_mul p256_group P1 P2)
+                               (bignum_triple_from_memory(p3,4) s))
           (MAYCHANGE [PC; X0; X1; X2; X3; X4; X5; X6; X7; X8; X9; X10;
                       X11; X12; X13; X14; X15; X16; X17] ,,
            MAYCHANGE SOME_FLAGS ,,
@@ -1943,46 +2003,55 @@ let P256_MONTJMIXADD_CORRECT = time prove
   DISCARD_STATE_TAC "s21" THEN
   DISCARD_MATCHING_ASSUMPTIONS [`nonoverlapping_modulo a b c`] THEN
 
-  MAP_EVERY X_GEN_TAC
-   [`x1':int`; `y1':int`; `z1':int`; `x2':int`; `y2':int`; `z2':int`] THEN
-  DISCH_THEN(CONJUNCTS_THEN2 ASSUME_TAC MP_TAC) THEN
-  GEN_REWRITE_TAC I [IMP_CONJ] THEN DISCH_THEN SUBST_ALL_TAC THEN
-  REPLICATE_TAC 2 (DISCH_THEN(CONJUNCTS_THEN2 ASSUME_TAC MP_TAC)) THEN
-  REWRITE_TAC[tripled; paired; nistp256_encode; montgomery_encode; PAIR_EQ] THEN
-  DISCH_THEN(REPEAT_TCL CONJUNCTS_THEN
-   (STRIP_ASSUME_TAC o MATCH_MP unilemma2)) THEN
-
+  MAP_EVERY X_GEN_TAC [`P1:(int#int)option`; `P2:(int#int)option`] THEN
+  REWRITE_TAC[represents_p256; represents2_p256; tripled; paired] THEN
+  REWRITE_TAC[montgomery_decode; INT_OF_NUM_CLAUSES; INT_OF_NUM_REM] THEN
+  STRIP_TAC THEN
   REPEAT(FIRST_X_ASSUM(MP_TAC o check (is_imp o concl))) THEN
   REPEAT(ANTS_TAC THENL
    [REWRITE_TAC[p_256] THEN RULE_ASSUM_TAC(REWRITE_RULE[p_256]) THEN
     CONV_TAC NUM_REDUCE_CONV THEN ASM BOUNDER_TAC[];
     (DISCH_THEN(STRIP_ASSUME_TAC o MATCH_MP unilemma0) ORELSE
-     DISCH_THEN(STRIP_ASSUME_TAC o MATCH_MP unilemma1))]) THEN
+     DISCH_THEN(STRIP_ASSUME_TAC o MATCH_MP unilemma1) ORELSE
+     STRIP_TAC)]) THEN
+  ASM_REWRITE_TAC[] THEN
+  MAP_EVERY (MP_TAC o C SPEC unreplemma)
+   [`y2:num`; `x2:num`; `z1:num`; `y1:num`; `x1:num`] THEN
+  MAP_EVERY (fun t -> ABBREV_TAC t THEN POP_ASSUM(K ALL_TAC))
+   [`x1d = inverse_mod p_256 (2 EXP 256) * x1`;
+    `y1d = inverse_mod p_256 (2 EXP 256) * y1`;
+    `z1d = inverse_mod p_256 (2 EXP 256) * z1`;
+    `x2d = inverse_mod p_256 (2 EXP 256) * x2`;
+    `y2d = inverse_mod p_256 (2 EXP 256) * y2`] THEN
+  ASM_REWRITE_TAC[] THEN REPEAT DISCH_TAC THEN
   REPEAT(FIRST_X_ASSUM(K ALL_TAC o GEN_REWRITE_RULE I [GSYM NOT_LE])) THEN
-
   RULE_ASSUM_TAC(REWRITE_RULE
    [num_congruent; GSYM INT_OF_NUM_CLAUSES; GSYM INT_OF_NUM_REM]) THEN
   RULE_ASSUM_TAC(REWRITE_RULE[GSYM INT_REM_EQ]) THEN
-  RULE_ASSUM_TAC(ONCE_REWRITE_RULE[GSYM INT_SUB_REM; GSYM INT_ADD_REM]) THEN
+  RULE_ASSUM_TAC(CONV_RULE INT_REM_DOWN_CONV) THEN
   RULE_ASSUM_TAC(REWRITE_RULE[INT_POW_2]) THEN
-  RULE_ASSUM_TAC(GEN_REWRITE_RULE (RAND_CONV o TRY_CONV) [lemont]) THEN
-
-  ASM_REWRITE_TAC[jacobian_add; nistp256] THEN
-  ASM_REWRITE_TAC[GSYM nistp256] THEN
-  REWRITE_TAC[INTEGER_MOD_RING_CLAUSES] THEN
-  CONV_TAC INT_REDUCE_CONV THEN ASM_REWRITE_TAC[] THEN
-  CONV_TAC(TOP_DEPTH_CONV let_CONV) THEN
+  RULE_ASSUM_TAC(ONCE_REWRITE_RULE[GSYM INT_ADD_REM; GSYM INT_SUB_REM]) THEN
+  RULE_ASSUM_TAC(ONCE_REWRITE_RULE[lemont; demont]) THEN
+  ASM_REWRITE_TAC[GSYM INT_OF_NUM_CLAUSES; GSYM INT_OF_NUM_REM] THEN
+  REWRITE_TAC[INT_REM_REM] THEN
+  REWRITE_TAC[pumont; dismont; unmont] THEN
+  FIRST_X_ASSUM(MP_TAC o GEN_REWRITE_RULE LAND_CONV [GSYM
+    weierstrass_of_affine_p256]) THEN
+  FIRST_X_ASSUM(MP_TAC o
+    check(can (term_match [] `weierstrass_of_jacobian f j = p`) o concl)) THEN
+  REWRITE_TAC[IMP_IMP] THEN
+  ASM_CASES_TAC `&z1d rem &p_256 = &0` THENL
+   [ASM_REWRITE_TAC[weierstrass_of_jacobian; INTEGER_MOD_RING_CLAUSES];
+    ALL_TAC] THEN
+  DISCH_THEN(fun th -> STRIP_ASSUME_TAC th THEN MP_TAC th) THEN
+  MATCH_MP_TAC weierstrass_of_jacobian_p256_add THEN ASM_REWRITE_TAC[] THEN
+  ASM_REWRITE_TAC[jacobian_add_unexceptional; nistp256;
+                  INTEGER_MOD_RING_CLAUSES] THEN
+  REWRITE_TAC[p_256] THEN CONV_TAC INT_REDUCE_CONV THEN
+  REWRITE_TAC[GSYM p_256] THEN
+  CONV_TAC(TOP_DEPTH_CONV let_CONV) THEN REWRITE_TAC[PAIR_EQ] THEN
   CONV_TAC INT_REM_DOWN_CONV THEN
-  REWRITE_TAC[tripled; paired; nistp256_encode; montgomery_encode] THEN
-  REWRITE_TAC[PAIR_EQ; GSYM INT_OF_NUM_EQ; nintlemma] THEN
-  CONV_TAC INT_REM_DOWN_CONV THEN
-
-  ASM_REWRITE_TAC[pumont; INT_REM_REM; GSYM INT_ADD_LDISTRIB;
-                GSYM INT_ADD_LDISTRIB; GSYM INT_SUB_LDISTRIB;
-                INT_SUB_REM; INT_ADD_REM] THEN
-
-  REPEAT CONJ_TAC THEN AP_THM_TAC THEN AP_TERM_TAC THEN AP_TERM_TAC THEN
-  INT_ARITH_TAC);;
+  REPEAT CONJ_TAC THEN AP_THM_TAC THEN AP_TERM_TAC THEN INT_ARITH_TAC);;
 
 let P256_MONTJMIXADD_SUBROUTINE_CORRECT = time prove
  (`!p3 p1 t1 p2 t2 pc stackpointer returnaddress.
@@ -2000,18 +2069,11 @@ let P256_MONTJMIXADD_SUBROUTINE_CORRECT = time prove
                   bignum_triple_from_memory (p1,4) s = t1 /\
                   bignum_pair_from_memory (p2,4) s = t2)
              (\s. read PC s = returnaddress /\
-                  (!x1 y1 z1 x2 y2 z2.
-                        ~(z1 = &0) /\ z2 = &1 /\
-                        ~(jacobian_eq (integer_mod_ring p_256)
-                                      (x1,y1,z1) (x2,y2,z2)) /\
-                        ~(jacobian_eq (integer_mod_ring p_256)
-                                      (jacobian_neg nistp256 (x1,y1,z1))
-                                      (x2,y2,z2)) /\
-                        t1 = tripled nistp256_encode (x1,y1,z1) /\
-                        t2 = paired nistp256_encode (x2,y2)
-                        ==> bignum_triple_from_memory(p3,4) s =
-                            tripled nistp256_encode
-                             (jacobian_add nistp256 (x1,y1,z1) (x2,y2,z2))))
+                  !P1 P2. represents_p256 P1 t1 /\
+                          represents2_p256 P2 t2 /\
+                          ~(P1 = NONE) /\ ~(P1 = P2)
+                          ==> represents_p256 (group_mul p256_group P1 P2)
+                               (bignum_triple_from_memory(p3,4) s))
           (MAYCHANGE_REGS_AND_FLAGS_PERMITTED_BY_ABI ,,
            MAYCHANGE [memory :> bytes(p3,96);
                       memory :> bytes(word_sub stackpointer (word 192),192)])`,
